compiler/backend/stateLangScript.sml
@@ -400,7 +400,7 @@ Definition sinterp_def:
         | Err => Ret' Error
         | Div => Div'
         | Act a k' st' =>
-            Vis' a (λy. value (Closure NONE [] $ Lit $ Str y) st' k' ))
+            Vis' a (λy. value (Closure NONE [] $ Delay $ Lit $ Str y) st' k' ))
       ((λ_ ret. STRLEN ret ≤ max_FFI_return_size),
        pure_semantics$FinalFFI,
        λs. pure_semantics$FinalFFI s pure_semantics$FFI_failure)
